agda/plfa/Lam/Canonical.agda
@@ -1,0 +1,40 @@
+module Lam.Canonical where
+
+open import Data.Nat
+open import Data.Bool
+
+open import Lam.Id
+open import Lam.Op
+open import Lam.Type
+open import Lam.Value
+open import Lam.Typing
+open import Lam.Syntax
+open import Lam.Context
+open import Lam.Reduction
+
+
+infix 4 Canonical_∶_
+
+data Canonical_∶_ : Term → Type → Set where
+
+  C-ƛ : ∀ {x : Id} {A B : Type} {N : Term}
+    →  ∅ , x ∶ A ⊢ N ∶ B
+      --------------------
+    → Canonical (ƛ x ⇒ N) ∶ A ⇒ B
+
+  C-zero :
+      ---------------------
+      Canonical `zero ∶ `ℕ
+
+  C-suc : ∀ {V : Term}
+    →  Canonical V ∶ `ℕ
+      --------------------
+    → Canonical (`suc V) ∶ `ℕ
+
+  C-Num : ∀ {n : ℕ}
+      ---------------------
+    → Canonical (eNum n) ∶ `Num
+
+  C-Bool : ∀ {b : Bool}
+      ----------------------
+    → Canonical (eBool b) ∶ `𝔹
